CoqOfRust/links/M.v
@@ -935,9 +935,9 @@ Module Run.
   | Let
       (ty : Ty.t) (e : M) (k : Value.t + Exception.t -> M)
       (of_ty : OfTy.t ty) :
-    let Output' : Set := Ref.t Pointer.Kind.Raw (OfTy.get_Set of_ty) in
+    let Output' : Set := OfTy.get_Set of_ty in
     {{ e 🔽 R, Output' }} ->
-    (forall (value_inter : Output.t R Output'),
+    (forall (value_inter : Output.t R (Ref.t Pointer.Kind.Raw Output')),
       {{ k (Output.to_value value_inter) 🔽 R, Output }}
     ) ->
     {{ LowM.Let ty e k 🔽 R, Output }}
@@ -996,13 +996,13 @@ Module LowM.
   Inductive t (R Output : Set) : Set :=
   | Pure (value : Output.t R Output)
   | CallPrimitive {A : Set} (primitive : Primitive.t A) (k : A -> t R Output)
-  | Let {A : Set} (e : t R A) (k : Output.t R A -> t R Output)
   | Call {A : Set} (e : t A A) (k : SuccessOrPanic.t A -> t R Output)
+  | Let {A : Set} `{Link A} (e : t R A) (k : Output.t R (Ref.t Pointer.Kind.Raw A) -> t R Output)
   | Loop {A : Set} (body : t R A) (k : Output.t R A -> t R Output).
   Arguments Pure {_ _}.
   Arguments CallPrimitive {_ _ _}.
-  Arguments Let {_ _ _}.
   Arguments Call {_ _ _}.
+  Arguments Let {_ _ _ _}.
   Arguments Loop {_ _ _}.
 End LowM.
 
@@ -1108,12 +1108,12 @@ Proof.
     end.
   }
   { (* Let *)
-    eapply LowM.Let. {
+    eapply (LowM.Let (A := Output')). {
       exact (evaluate _ _ _ _ _ run).
     }
     intros output'; eapply evaluate.
     match goal with
-    | H : forall _ : Output.t _ Output', _ |- _ => apply (H output')
+    | H : forall _ : Output.t _ (Ref.t Pointer.Kind.Raw Output'), _ |- _ => apply (H output')
     end.
   }
   { (* Loop *)
